---
title: "CUNY SPS Discussion 14"
author: "Chinedu Onyeka"
date: "2023-11-28"
output: html_document
---

```{r setup, include=FALSE}
knitr::opts_chunk$set(echo = TRUE)
```

<center><h3>Question</h3></center>
Chapter 8.8, Pg 496 Question 7
Find a formula for the $n^{th}$ term of the Taylor series for $f(x)$.  
$f(x) = cosx,\ c = \pi/2$  

<h3>Solution </h3> 

Taylor Series is defined as 
$$
\begin{split}
f(x) &= \sum\limits_{n=0}^{\infty}\frac{f^{(n)}(a)}{n!}(x-a)^n \\
 &= f(a) + f'(a)(x-a) + \frac{f''(a)}{2!}(x-a)^2 + \frac{f'''(a)}{3!}(x-a)^3 + \frac{f'^v(a)}{4!}(x-a)^4 + \  ... 
\end{split}
$$

Find the first 5 derivatives of f(x):  
$$
\begin{split}
f(x) &= cosx; \ => f^0(\pi/2) = cos(\pi/2) = 0, \\
f'(x) &= -sinx;\ => f'(\pi/2) = -sin(\pi/2) = -1, \\
f''(x) &= -cosx;\ => f''(\pi/2) = -cos(\pi/2) = 0, \\
f'''(x) &= sinx;\  => f'''(\pi/2) = sin(\pi/2) = 1, \\
f'^v(x) &= cosx;\  => f'^v(\pi/2) = cos(\pi/2) = 0, \\
f^v(x) &= -sinx;\  => f^v(\pi/2) = -sin(\pi/2) = -1
\end{split}
$$

Following the definition of the Taylor's series given above,   
$$
\begin{split}
f(x) &= \frac{f^0(c)}{0!}(x-c)^0 + \frac{f'(c)}{1!}(x-c)^1 + \frac{f''(c)}{2!}(x-c)^2 + \frac{f'''(c)}{3!}(x-c)^3 +                        \frac{f'^v(c)}{4!}(x-c)^4 + \frac{f^v(c)}{5!}(x-c)^5 + \ ...\\
 &= \frac{0}{0!}(x-\pi/2)^0 + \frac{-1}{1!}(x-\pi/2)^1 + \frac{0}{2!}(x-\pi/2)^2 + \frac{1}{3!}(x-\pi/2)^3 +                          \frac{0}{4!}(x-\pi/2)^4 + \frac{-1}{5!}(x-\pi/2)^5 + \ ...\\
&= - (x-\pi/2)  + \frac{(x-\pi/2)^3}{3!} - \frac{(x-\pi/2)^5}{5!} + \ ... \\
&= \sum\limits_{n=0}^{\infty} (-1)^{n+1} \frac{(x-\pi/2)^{2n+1}}{(2n+1)!}
\end{split}
$$
<br>

Therefore, the formula for the $n^{th}$ term of the Taylor series for $cosx$ where $c = \pi/2$ is given by:  
$f(n) = \sum\limits_{n=0}^{\infty} (-1)^{n+1} \frac{(x-\pi/2)^{2n+1}}{(2n+1)!}$
